PQueue example complete

examples/priority_queue/PQueueA.v
@@ -1,7 +1,7 @@
 Require Import CRIS.
 Require Import MemHeader MemA MemTactics.
 Require Import SchHeader SchI SchA SchTactics.
-Require Import StackHeader StackA StackIA.
+Require Import StackHeader StackA.
 Require Import PQueueHeader PQueueI.
 From iris.algebra Require Import excl_auth.
 
@@ -25,9 +25,9 @@ Section definitions.
       (n : nat) (γq : gname) (range : nat) (qb : mblock) (qofs : ptrofs)
       (entries : list (val * gname))
       : GTerm.t n := (
-    <own> γq (excl_auth_frag entries) ∗
+    sown γq (excl_auth_frag entries) ∗
     (qb, qofs) ↦ Vint range ∗
-    [∗ n list] i ↦ x ∈ entries, (qb, qofs + i + 1)%Z ↦ x.1
+    [∗ list] i ↦ x ∈ entries, (qb, qofs + i + 1)%Z ↦ x.1
   )%SAT.
   Definition queue_inv
       (n : nat) (γq : gname) (range : nat) (qb : mblock) (qofs : ptrofs) 
@@ -38,15 +38,15 @@ Section definitions.
     [∗ list] i ↦ x ∈ entries, (qb, qofs + Z.of_nat i + 1)%Z ↦ x.1
   )%I.
   Global Instance queue_inv_SLRed n γq range qb qofs entries :
-    SLRed (syn_queue_inv n γq range qb qofs entries) (queue_inv n γq range qb qofs entries).
-  Proof. rewrite /syn_queue_inv /queue_inv; econs; rewrite SLRed_eq //. Qed.
+    SLRed n (syn_queue_inv n γq range qb qofs entries) (queue_inv n γq range qb qofs entries).
+  Proof. solve_base_sl_red. Qed.
 
   Definition syn_is_queue (n : nat) (γq : gname) (range : nat) (q : val) : GTerm.t n := (
     ∃ (qb : τ{mblock}) (qofs : τ{ptrofs}), ⌜q = Vptr (qb, qofs)⌝ ∗
       ∃ (entries : τ{list (val * gname)}),
         ⌜length entries = range⌝ ∗
-        syn_inv n queueN (syn_queue_inv n γq range qb qofs entries) ∗
-        [∗ n list] i ↦ e ∈ entries, syn_is_stack (stackN N) e.2 e.1 n
+        syn_inv queueN (syn_queue_inv n γq range qb qofs entries) ∗
+        [∗ list] i ↦ e ∈ entries, syn_is_stack (stackN N) e.2 e.1 n
   )%SAT.
   Definition is_queue (n : nat) (γq : gname) (range : nat) (q : val) : iProp Σ :=
     ∃ (qb : mblock) (qofs : ptrofs), ⌜q = Vptr (qb, qofs)⌝ ∗
@@ -55,11 +55,8 @@ Section definitions.
         inv n queueN (syn_queue_inv n γq range qb qofs entries) ∗
         [∗ list] i ↦ e ∈ entries, is_stack (stackN N) e.2 e.1 n.
   Global Instance is_queue_SLRed n γq q range :
-    SLRed (syn_is_queue n γq q range) (is_queue n γq q range).
-  Proof.
-    rewrite /syn_is_queue /is_queue; econs; rewrite SLRed_eq //. do 4 (f_equiv; ii); ss.
-    rewrite inv_red //.
-  Qed.
+    SLRed n (syn_is_queue n γq q range) (is_queue n γq q range).
+  Proof. solve_base_sl_red. Qed.
   Global Instance is_queue_persistent n γq q range :
     Persistent (is_queue n γq q range).
   Proof. apply _. Qed.
@@ -75,7 +72,7 @@ Module PQueueA. Section PQueueA.
   Context `{!stackG StackM.jobID StackM.retID, !queueG}.
   Context (N : namespace).
 
-  Definition scopes : list string := [].
+  Definition scopes : gmultiset string := ∅.
 
   Definition new_spec : fspec :=
     fspec_sch (↑N)
@@ -102,7 +99,7 @@ Module PQueueA. Section PQueueA.
     𝒴;;; fbody_trivial ()↑.
 
   Definition add : Any.t → itree crisE Any.t :=
-    atomic_body (from_fspec add_spec)
+    atomic_body (add_spec)
       (λ '(_, _, (γq, _, priority, v)) _,
         𝒴;;;
         l <- trigger (Take (list (list val)));;
@@ -113,7 +110,7 @@ Module PQueueA. Section PQueueA.
         Ret Vundef↑).
 
   Definition remove_min : Any.t → itree crisE Any.t :=
-    atomic_body (from_fspec remove_min_spec)
+    atomic_body (remove_min_spec)
       (λ '(_, _, (γq, range)) _,
         𝒴;;;
         'ret : val <- ITree.iter (λ n : nat,
@@ -136,61 +133,60 @@ Module PQueueA. Section PQueueA.
         𝒴;;;
         Ret ret↑).
 
-  Definition fnsems : fnsems_type :=
-    [(Some PQueueHdr.new, (true, wmask_all, scopes, (Some new_spec, new)));
-     (Some PQueueHdr.add, (true, wmask_all, scopes, (None, add)));
-     (Some PQueueHdr.remove_min, (true, wmask_all, scopes, (None, remove_min)))].
+  Definition fnsems : fnsemmap :=
+    {[Some PQueueHdr.new := Some (msk_scp scopes msk_true, (fsp_some new_spec, new));
+      Some PQueueHdr.add := Some (msk_scp scopes msk_true, (None, add));
+      Some PQueueHdr.remove_min := Some (msk_scp scopes msk_true, (None, remove_min))]}.
 
   Program Definition Mod : SMod.t := {|
     SMod.scopes := scopes;
     SMod.fnsems := fnsems;
-    SMod.initial_st := [];
+    SMod.initial_st := ∅;
   |}.
-  Solve All Obligations with prove_scope.
-  Next Obligation. prove_nodup. Qed.
+  Solve All Obligations with mod_tac.
 
-  Definition t sp := Seal.sealing CRIS (SMod.to_mod sp Mod).
+  Definition t sp := SMod.to_mod sp Mod.
 End PQueueA. End PQueueA.
 
 Module PQueueIA. Section PQueueIA.
   Context `{!crisG Γ Σ α β τ _S _I, !concG, !newschG, !memG}.
   Context `{!stackG StackM.jobID StackM.retID, !queueG}.
 
-  Context (N : namespace) (sp : sp_type).
-  Context (Hsch : sp_incl (SchA.sp [] (↑N)) sp).
+  Context (N : namespace) (sp sp_user : specmap).
+  Context (Hsch : (SchA.sp sp_user (↑N)) ⊆ sp).
 
   Definition init_cond : iProp Σ := emp%I.
 
-  Local Definition sp_stack : sp_type := to_sp (SchA.sp  [] (↑(stackN N))).
-  Local Definition StackA := StackA.t (stackN N) sp_stack.
-  Local Definition PQueueI := PQueueI.t      ★ (StackA ★ SchI.t ★ MemA.t sp_none).
-  Local Definition PQueueA := PQueueA.t N sp ★ (StackA ★ SchI.t ★ MemA.t sp_none).
+  (* Local Definition sp_stack : specmap := SchA.sp ∅ (↑(stackN N)). *)
+  Local Definition StackA := StackA.t (stackN N) (SchA.sp ∅ (↑(stackN N))).
+  Local Definition PQueueA := PQueueA.t N sp ★ (StackA ★ SchI.t ★ MemA.t sp).
+  Local Definition PQueueI := PQueueI.t      ★ (StackA ★ SchI.t ★ MemA.t sp).
   Local Definition IstFull := IstProd (IstSB (Mod.scopes (PQueueA.t N sp)) IstTrue) IstEq.
 
-  Lemma new_simF : ISim.sim_fun open PQueueA PQueueI init_cond IstFull (Some PQueueHdr.new).
+  Lemma new_simF : ISim.sim_fun open PQueueA PQueueI IstFull (Some PQueueHdr.new).
   Proof.
-    init_simF.
-    steps_l. iDestruct "ASM" as "[TID [[-> %Hn] ->]]".
-    rename _q3 into stid, _q4 into mtid, _q5 into n, _q6 into range.
+    iStartSim.
+    steps_l. destruct _q as [[stid mtid] [n range]].
+    iDestruct "ASM" as "[TID [-> [-> %Hn]]]".
 
-    steps_r. hss_r. steps_r. sch_yield_ir. steps_r. sch_yield_ir. steps_r.
+    steps_r. hss_r. steps_r. rewrite /PQueueA.new. steps_l.
+    sch_yield_ir "IST" "TID". steps_r. sch_yield_ir "IST" "TID". steps_r.
     iApply wsim_mem_alloc; [try prove_inline_cond|try prove_sb_cond|ss|unfold_cris_defs].
     { lia. }
-    iIntros (queueb) "↦queue". steps_r. hss_r. steps_r. sch_yield_ir. steps_r.
-    sch_yield_ir. steps_r.
+    iIntros (queueb) "↦queue". steps_r. hss_r. steps_r.
+    sch_yield_ir "IST" "TID". steps_r.
+    sch_yield_ir "IST" "TID". steps_r.
     rewrite (comm Z.add) Z2Nat.inj_add //; try lia.
-    rewrite repeat_app /=; iDestruct "↦queue" as "[↦range ↦queue]".
-    iApply (wsim_mem_store with "[↦range]");
-        [try prove_inline_cond|try prove_sb_cond|..|unfold_cris_defs]; iFrame.
-    iIntros "↦range". steps_r. hss_r. steps_r.
+    rewrite replicate_add /=; iDestruct "↦queue" as "[↦range ↦queue]".
+    store_r "↦range". steps_r. hss_r. steps_r.
 
     iApply wsim_yy_y. iApply wsim_bind.
     instantiate (1:=(λ '(st_src, _) '(st_tgt, _),
-      IstFull st_src st_tgt ∗ Tid stid mtid ∗ winv (↑N, ↑N) ∗
+      IstFull st_src st_tgt ∗ Tid mtid stid ∗ winv (↑N, ↑N) ∗
       ∃ γq, is_queue N n γq range (Vptr (queueb, 0%Z)) ∗
       queue_contents γq (repeat [] range))%I).
     iSplitL "↦range ↦queue IST TID".
-    { rewrite ?Nat2Z.id. erewrite <-(bind_ret_r (SB.sandbox _ _ _ _)).
+    { rewrite ?Nat2Z.id.
       iAssert (∃ entries,
         ⌜length entries = range⌝ ∗
         [∗ list] i ↦ v ∈ entries,
@@ -202,24 +198,24 @@ Module PQueueIA. Section PQueueIA.
       { iExists (repeat (Vundef, 1%positive) range).
         rewrite repeat_length; iSplit; first done. clear Hn.
         iInduction (range) as [|range]; first ss.
-        rewrite -Nat.add_1_r ?repeat_app /= ?big_sepL_app /=; case_decide; try lia.
+        rewrite -Nat.add_1_r !replicate_add !repeat_app /= ?big_sepL_app /=; case_decide; try lia.
         rewrite ?repeat_length /=.
         iDestruct "↦queue" as "[↦queues [↦queue _]]".
         iPoseProof ("IHrange" with "[↦queues]") as "↦queues"; eauto. iFrame.
-        rewrite Nat.add_0_r Z.add_1_r Nat2Z.inj_succ; iFrame.
+        rewrite length_replicate Nat.add_0_r Z.add_1_r Nat2Z.inj_succ; iFrame.
       }
       set (var := range).
       rewrite {1 2 3 4}/var.
       replace (0%Z) with (range - var)%Z by lia.
-      rewrite {1 6}Z.sub_diag.
+      rewrite {5}Z.sub_diag.
        (* rewrite {1 3 5 6 7 8 9 10 11 12 13 14 15 17}/var. *)
       iAssert (⌜var ≤ range⌝)%I as "#Hvar"; first (iPureIntro; lia).
       generalize var. clear var. iIntros (var).
       iInduction (var) as [|var] forall (st_src st_tgt).
       { unfold_iter_r. steps_r.
-        erewrite <-(bind_ret_r (SB.sandbox _ _ _ _)). steps_l.
-        sch_yield_ir. steps_r.
-        sch_yield_l. ss.
+        add_ret_l. steps_l.
+        sch_yield_ir "IST" "TID". steps_r.
+        sch_yield_l.
         iDestruct "↦queue" as "[%entries [% ↦queues]]". rewrite Z.sub_0_r.
         iAssert ([∗ list] i ↦ v ∈ entries,
           is_stack (stackN N) v.2 v.1 n ∗ (queueb, Z.of_nat i + 1)%Z ↦ v.1 ∗ stack_content v.2 [])%I
@@ -235,12 +231,13 @@ Module PQueueIA. Section PQueueIA.
         iMod (inv_alloc (syn_queue_inv n γq range queueb 0 entries) _ _ _ (queueN N)
           with "[◯q ↦queues ↦range]") as "#Qinv"; eauto.
         { apply nclose_subseteq. }
-        { rewrite SLRed_eq /queue_inv; iFrame; ss. }
-        iApply wsim_unfold; iIntros "W". step. iFrame "IST TID W". iExists γq. iSplitR.
+        { solve_base_sl_red; iFrame. }
+        step. iFrame. iSplitR.
         { iExists _, _; iSplit; first done.
           iExists entries; iSplit; first done. iSplit; done.
         }
-        iExists _; iFrame; ss. rewrite repeat_length; iSplit; first done.
+        subst range.
+        rewrite repeat_length; iSplit; first done.
         iApply (big_sepL_impl with "↦stack_contents").
         iIntros "!> %%%Hlookup S"; set (elem := _ !!! _).
         assert (Hin : elem ∈ repeat [] (length entries)).
@@ -250,18 +247,16 @@ Module PQueueIA. Section PQueueIA.
 
       iPoseProof "Hvar" as "%".
       unfold_iter_r. steps_r.
-      sch_yield_ir. steps_r.
+      add_ret_l. sch_yield_ir "IST" "TID". steps_r.
+
       (* stack allocation *)
       inline_r. force_r (stid, mtid, n). forces_r.
       iFrame. iSplit; eauto.
-      steps_r. hss_r. steps_r. steps_l. steps_r. sch_yield_ii.
-      { apply sp_incl_to_sp; rewrite /SchA.sp; unseal CRIS; ss; prove_nodup. }
-      { eapply union_difference, nclose_subseteq. }
-      { set_solver. }
-      steps_r. iDestruct "GRT" as "[TID [[%stack [%γs [-> [#is_stack stack]]]] %]]".
+      steps_r. hss_r. steps_r.
+      sch_yield_ii "IST".
+      steps_r. iDestruct "GRT" as "[TID [-> [%stack [%γs [-> [#is_stack stack]]]]]]".
       hss_r. steps_r.
-      rewrite ?copset_diff_union; try eapply nclose_subseteq.
-      sch_yield_ir. steps_r.
+      sch_yield_ir "IST" "TID". steps_r.
 
       iDestruct "↦queue" as "[%entries [%Hentries ↦queue]]".
       hexploit (lookup_lt_is_Some_2 entries (range - S var)); first lia; intros [p Hp].
@@ -273,18 +268,19 @@ Module PQueueIA. Section PQueueIA.
       { rewrite list_lookup_insert //; lia. }
       case_decide; last lia.
 
-      iApply (wsim_mem_store with "[↦queue]");
-        [try prove_inline_cond|try prove_sb_cond|..|unfold_cris_defs].
-      { rewrite Nat2Z.inj_sub //. }
-      iIntros "↦queue". steps_r. hss_r. steps_r.
+      rewrite Nat2Z.inj_sub //.
+      store_r "↦queue". steps_r. hss_r. steps_r.
       replace (length entries - S var + 1)%Z with (length entries - var)%Z by lia.
-      sch_yield_ir. steps_r.
+      sch_yield_ir "IST" "TID". steps_r.
 
+      replace (range - S var + 1 + 1)%Z with (range - var + 1)%Z by lia.
+      rewrite bind_ret_r.
       iApply ("IHvar" with "[] ↦range IST TID [-]").
       { iIntros "!>"; iPureIntro; lia. }
       iExists (<[length entries - S var := (stack, γs)]> entries); iSplit.
       { rewrite length_insert //. }
 
+      subst range.
       iApply ("↦close" with "[] [↦queue stack]").
       { iModIntro; iIntros (??) "%% H"; do 2 case_decide; try lia; iFrame. }
       { case_decide; try lia. ss.
@@ -296,47 +292,41 @@ Module PQueueIA. Section PQueueIA.
     (* continuation *)
     clear_st. iIntros (st_s _ st_t _) "[IST [TID [W [%γq [#qinv queue]]]]]".
     iApply wsim_fold; iFrame "W".
-    steps_r. sch_yield_ir. steps_r.
+    steps_r. sch_yield_ir "IST" "TID". steps_r.
     sch_yield_l. forces_l. iFrame. iSplit; eauto. step. iSplit; done.
   Unshelve. all: eauto.
   (*SLOW*)Qed.
 
-  Lemma add_simF : ISim.sim_fun open PQueueA PQueueI init_cond IstFull (Some PQueueHdr.add).
+  Lemma add_simF : ISim.sim_fun open PQueueA PQueueI IstFull (Some PQueueHdr.add).
   Proof.
-    init_simF.
-    steps_l. iDestruct "ASM" as "[TID [[%n [%q [[-> %] #[%queueb [%queueofs [-> is_queue]]]]]] _]]".
-    rename _q2 into stid, _q3 into mtid, _q5 into v, _q7 into priority, _q8 into γq, _q9 into range.
+    iStartSim. rewrite /PQueueA.add /atomic_body.
+    steps_l. destruct _q as [[stid mtid] [[[γq range] priority] v]].
+    iDestruct "ASM" as "[TID [_ [%n [%q [[-> %] #[%queueb [%queueofs [-> is_queue]]]]]]]]".
 
-    steps_r. hss_r. steps_r. sch_yield_ir. steps_r. sch_yield_ir. steps_r.
+    steps_r. hss_r. steps_r.
+    sch_yield_ir "IST" "TID". steps_r. sch_yield_ir "IST" "TID". steps_r.
     iDestruct "is_queue" as "[%entries [%Hlen [#qinv #stacks]]]".
-    iInv "qinv" as "inv" "close". rewrite SLRed_eq.
-    iDestruct "inv" as "[◯entries [↦range ↦]]".
+    iInv "qinv" as "[◯entries [↦range ↦]]" "close".
     iCombine "stacks" "↦" as "↦"; rewrite -big_sepL_sep.
     hexploit (lookup_lt_is_Some_2 entries priority); first lia; intros [[stack γs] Hstack].
     iPoseProof (big_sepL_lookup_acc_impl priority with "↦") as "[[#stack ↦] ↦s]"; eauto; s.
 
-    iApply (wsim_mem_load with "[↦]");
-      [try prove_inline_cond|try prove_sb_cond|ss|unfold_cris_defs].
-    iIntros "↦". steps_r. hss_r. steps_r.
+    load_r "↦". steps_r. hss_r. steps_r.
     iMod ("close" with "[↦s ↦range ↦ ◯entries]") as "_".
-    { iFrame. iApply ("↦s" with "[] [↦]"); iFrame.
-      iIntros "!> %%%% [?$]".
-    }
-    sch_yield_ir. steps_r.
+    { iFrame. iApply ("↦s" with "[] [↦]"); iFrame. iIntros "!> %%%% [?$]". }
+    sch_yield_ir "IST" "TID". steps_r.
     
     (* stack push *)
-    inline_r. steps_r. force_r (_, _, (n, stack, v, γs)); forces_r. iFrame. iSplit; eauto. steps_r.
-    sch_yield_ii.
-    { apply sp_incl_to_sp; rewrite /SchA.sp; unseal CRIS; ss; prove_nodup. }
-    { eapply union_difference, nclose_subseteq. }
-    { set_solver. }
+    inline_r. rewrite /StackA.push /atomic_body.
+    steps_r. force_r (_, _, (n, stack, v, γs)); forces_r. iFrame. iSplit; eauto. steps_r.
+    sch_yield_ii "IST".
     steps_r.
 
     (* atomic update *)
-    sch_yield_l. steps_l. rename _q into queue. set (entry := queue !!! priority).
-    iDestruct "ASM" as "[%entries' [%Hlen [● stack_contents]]]".
-    iInv "qinv" as "inv" "close". rewrite SLRed_eq.
-    iDestruct "inv" as "[◯ inv]". iCombine "●" "◯" gives %->%excl_auth_agree_L.
+    sch_yield_l. steps_l. sch_yield_l. steps_l.
+    rename _q into queue. set (entry := queue !!! priority).
+    iDestruct "ASM" as "[%entries' [%Hlen' [● stack_contents]]]".
+    iInv "qinv" as "[◯ inv]" "close". iCombine "●" "◯" gives %->%excl_auth_agree_L.
     iMod ("close" with "[◯ inv]") as "_"; first iFrame.
     iPoseProof (big_sepL_lookup_acc_impl priority with "stack_contents") as "[s contents]"; eauto.
 
@@ -345,102 +335,81 @@ Module PQueueIA. Section PQueueIA.
     { iExists entries; iFrame. rewrite length_insert; iSplit; first done.
       iApply ("contents" with "[] [GRT]").
       { iIntros "!> %k %y %Hky % s". rewrite list_lookup_total_insert_ne //. }
-      { s. rewrite list_lookup_total_insert // -Hlen; lia. }
+      { s. rewrite list_lookup_total_insert // -Hlen'; lia. }
     }
 
-    steps_l.
-    sch_yield_ii.
-    { apply sp_incl_to_sp; rewrite /SchA.sp; unseal CRIS; ss; prove_nodup. }
-    { eapply union_difference, nclose_subseteq. }
-    { set_solver. }
-    steps_r. hss_r. steps_r.
-    rewrite ?copset_diff_union; cycle 1.
-    { apply nclose_subseteq. }
+    steps_l. sch_yield_ii "IST". steps_r. hss_r. steps_r.
     iDestruct "GRT" as "[TID _]".
-    sch_yield_ir.
-    sch_yield_l. steps_l. force_l. iFrame. iSplit; eauto.
+    sch_yield_ir "IST" "TID".
+    sch_yield_l. steps_l. sch_yield_l. force_l. iFrame. iSplit; eauto.
     step. iFrame. done.
-    Unshelve. all: eauto.
   (*SLOW*)Qed.
 
-  Lemma remove_min_simF :
-    ISim.sim_fun open PQueueA PQueueI init_cond IstFull (Some PQueueHdr.remove_min).
+  Lemma remove_min_simF : ISim.sim_fun open PQueueA PQueueI IstFull (Some PQueueHdr.remove_min).
   Proof.
-    init_simF.
-    steps_l. iDestruct "ASM" as "[TID [[%n [%q [-> #[%queueb [%queueofs [-> Q]]]]]] _]]".
-    rename _q2 into stid, _q3 into mtid, _q4 into γq, _q5 into range.
+    iStartSim. rewrite /PQueueA.remove_min /atomic_body.
+    steps_l. destruct _q as [[stid mtid] [γq range]].
+    iDestruct "ASM" as "[TID [_ [%n [%q [-> #[%queueb [%queueofs [-> Q]]]]]]]]".
 
-    steps_r. hss_r. steps_r. sch_yield_ir. steps_r. sch_yield_ir. steps_r.
+    steps_r. hss_r. steps_r.
+    sch_yield_ir "IST" "TID". steps_r. sch_yield_ir "IST" "TID". steps_r.
     iDestruct "Q" as "[%entries [%Hlen [#queue_inv #stack_invs]]]".
-    iInv "queue_inv" as "inv" "close"; rewrite SLRed_eq.
-    iDestruct "inv" as "[◯ [↦range ↦queues]]".
+    iInv "queue_inv" as "[◯ [↦range ↦queues]]" "close".
 
     (* range load *)
-    iApply (wsim_mem_load with "[↦range]");
-      [try prove_inline_cond|try prove_sb_cond|ss|unfold_cris_defs].
-    iIntros "↦range". steps_r. hss_r. steps_r.
+    load_r "↦range". steps_r. hss_r. steps_r.
     iMod ("close" with "[◯ ↦range ↦queues]") as "_"; iFrame.
-    sch_yield_ir. steps_r. sch_yield_l. steps_l.
-    rewrite Nat2Z.id. set (var := length entries). rewrite {1 2 3 4 6}/var.
-    iAssert (⌜var ≤ length entries⌝)%I as "#Hvar"; first done.
-    replace (queueofs + 1)%Z with (queueofs + (length entries - var) + 1)%Z by lia.
-    generalize var; clear var; iIntros (var).
+    sch_yield_ir "IST" "TID". steps_r. sch_yield_l. steps_l. sch_yield_l. steps_l.
+    rewrite !Nat2Z.id.
+    iAssert (⌜range ≤ length entries⌝)%I as "#Hrange"; first by subst.
+    replace (queueofs + 1)%Z with (queueofs + (length entries - range) + 1)%Z by lia.
+    generalize range at 2 6 8 9. subst range. iIntros (var).
     iInduction (var) as [|var'] forall (st_src st_tgt).
     { unfold_iter_l; unfold_iter_r. steps_l; steps_r.
-      sch_yield_ir. steps_r. sch_yield_l. steps_l. force_l. iFrame; iSplit; eauto.
+      sch_yield_ir "IST" "TID". steps_r. sch_yield_l. steps_l. sch_yield_l.
+      force_l. iFrame; iSplit; eauto.
       step; iFrame; done.
     }
 
-    iPoseProof ("Hvar") as "%".
+    iPoseProof ("Hrange") as "%".
     unfold_iter_l. steps_l.
-    unfold_iter_r. steps_r. sch_yield_ir. steps_r.
+    unfold_iter_r. steps_r. sch_yield_ir "IST" "TID". steps_r.
 
     (* stack load *)
     rewrite -?Nat2Z.inj_sub; try lia.
     set (index := (length entries - S var')).
-    iInv "queue_inv" as "inv" "close"; rewrite SLRed_eq.
-    iDestruct "inv" as "[◯ [↦range ↦queues]]".
+    iInv "queue_inv" as "[◯ [↦range ↦queues]]" "close".
     hexploit (lookup_lt_is_Some_2 entries index); first lia; intros [[istack iγs] Hi].
     iPoseProof (big_sepL_lookup_acc _ _ index with "↦queues") as "[↦queue ↦queues]"; eauto; s.
     iPoseProof (big_sepL_lookup_acc _ _ index with "stack_invs") as "[stack _]"; eauto; s.
-
-    iApply (wsim_mem_load with "[↦queue]");
-      [try prove_inline_cond|try prove_sb_cond|ss|unfold_cris_defs].
-    iIntros "↦queue". steps_r. hss_r. steps_r.
+    load_r "↦queue". steps_r. hss_r. steps_r.
     iPoseProof ("↦queues" with "↦queue") as "↦queues".
     iMod ("close" with "[◯ ↦range ↦queues]") as "_"; iFrame.
-    sch_yield_ir. steps_r.
+    sch_yield_ir "IST" "TID". steps_r.
 
-    inline_r. steps_r. force_r (stid, mtid, (n, istack, iγs)). forces_r. iFrame. iSplit; eauto.
-    steps_r. sch_yield_ii.
-    { apply sp_incl_to_sp; rewrite /SchA.sp; unseal CRIS; ss; prove_nodup. }
-    { eapply union_difference, nclose_subseteq. }
-    { set_solver. }
-    steps_r.
+    inline_r. rewrite /StackA.pop /atomic_body. steps_r.
+    force_r (stid, mtid, (n, istack, iγs)). forces_r. iFrame. iSplit; eauto.
+    steps_r. sch_yield_ii "IST".
 
     (* atomic stack pop *)
     sch_yield_l. steps_l. rename _q into q. force_r (q !!! index). steps_r.
     iDestruct "ASM" as "[%entries' [%Hlenq [● ↦stacks]]]".
-    iInv "queue_inv" as "inv" "close". rewrite SLRed_eq.
-    iDestruct "inv" as "[◯ inv]". iCombine "●" "◯" gives %->%excl_auth_agree_L.
+    iInv "queue_inv" as "[◯ inv]" "close".
+    iCombine "●" "◯" gives %->%excl_auth_agree_L.
     iMod ("close" with "[◯ inv]") as "_"; first iFrame.
     iPoseProof (big_sepL_lookup_acc_impl index with "↦stacks") as "[↦stack ↦stacks]"; eauto; s.
     force_r; iFrame. steps_r. force_l. iSplitL "↦stacks GRT ●".
     { iFrame.
       iSplit; [rewrite length_insert //|].
       iApply ("↦stacks" with "[] [-]").
-      { iIntros "!> %%%%"; rewrite list_lookup_total_insert_ne //; iIntros "$". }
+      { iIntros "!> %%%%"; rewrite list_lookup_total_insert_ne //. iIntros "$". }
       { s; rewrite list_lookup_total_insert // -Hlenq; lia. }
     }
     steps_l.
 
     (* remainder *)
-    sch_yield_ii.
-    { apply sp_incl_to_sp; rewrite /SchA.sp; unseal CRIS; ss; prove_nodup. }
-    { eapply union_difference, nclose_subseteq. }
-    { set_solver. }
+    sch_yield_ii "IST".
     steps_r. hss_r. steps_r.
-    rewrite ?copset_diff_union; try apply nclose_subseteq.
 
     set (caseb :=
       match q !!! index with
@@ -449,11 +418,11 @@ Module PQueueIA. Section PQueueIA.
       | _ => false
       end
     ); destruct caseb eqn : Hcase.
-    { 
+    {
       set (case := match q !!! index with | [] => Vundef | _ => _ end).
       replace case with Vundef; cycle 1.
       { subst case caseb; destruct (q !!! index) as [|[?|?|]?]; ss. }
-      steps_r. iDestruct "GRT" as "[TID _]". sch_yield_ir. steps_r.
+      steps_r. iDestruct "GRT" as "[TID _]". sch_yield_ir "IST" "TID". steps_r.
       sch_yield_l. steps_l. clear case.
       set (case := match q !!! index with | Vint _ as v :: _ => _ | _ => _ end).
       replace case with (Ret (inl var') : itree crisE (nat + val)); cycle 1.
@@ -472,31 +441,29 @@ Module PQueueIA. Section PQueueIA.
     set (case := match v with | Vundef => _ | _ => _ end).
     replace case with (𝒴;;; Ret (inr v) : itree crisE (nat * Z + val)).
     2:{ subst case; des_ifs; ss. }
-    steps_r. iDestruct "GRT" as "[TID _]". sch_yield_ir. steps_r.
-    sch_yield_l. steps_l. sch_yield_l. force_l. iFrame. iSplit; eauto.
+    steps_r. iDestruct "GRT" as "[TID _]". sch_yield_ir "IST" "TID". steps_r.
+    sch_yield_l. steps_l. sch_yield_l. sch_yield_l. force_l. iFrame. iSplit; eauto.
     step. iFrame. done.
-  Unshelve. all: eauto.
   (*SLOW*)Qed.
 
-  Lemma sim :
-    ISim.t open PQueueA PQueueI emp IstFull.
+  Lemma sim : ISim.t open PQueueA PQueueI emp IstFull.
   Proof.
     init_sim.
-    { split; ss. iIntros "_"; iSplit; ss. }
     { apply new_simF. }
     { apply add_simF. }
     { apply remove_min_simF. }
+    { iIntros "_"; repeat iExists _; iPureIntro; ss. }
   Qed.
 End PQueueIA.
 Section ctxr.
   Context `{!crisG Γ Σ α β τ _S _I, !concG, !newschG, !memG}.
   Context `{!stackG StackM.jobID StackM.retID, !queueG}.
 
-  Lemma ctxr (N : namespace) (sp : sp_type) :
-    sp_incl (SchA.sp [] (↑N)) sp →
+  Lemma ctxr (N : namespace) (sp_user sp : specmap) :
+    SchA.sp sp_user (↑N) ⊆ sp →
     ctx_refines
-      (PQueueA.t N sp ★ StackA.t (stackN N) (sp_stack N) ★ SchI.t ★ MemA.t sp_none, emp%I)
-      (PQueueI.t ★ StackA.t (stackN N) (sp_stack N) ★ SchI.t ★ MemA.t sp_none, emp%I).
+      (PQueueA.t N sp ★ StackA.t (stackN N) (SchA.sp ∅ (↑(stackN N))) ★ SchI.t ★ MemA.t sp, emp%I)
+      (PQueueI.t      ★ StackA.t (stackN N) (SchA.sp ∅ (↑(stackN N))) ★ SchI.t ★ MemA.t sp, emp%I).
   Proof. intros Hsp. eapply main_adequacy, sim; eauto. Qed.
 End ctxr. End PQueueIA.
 
