examples/elimination_stack/StackA.v
@@ -2,7 +2,7 @@ Require Import CRIS.
 Require Import MemHeader MemA.
 Require Import SchHeader SchA.
 From CRIS.helping Require Import Header HelpingTactics.
-Require Import StackHeader IndefiniteDescription.
+Require Import StackHeader.
 
 Class stackG (jobID retID : Type) `{!crisG Γ Σ α β τ _S _I} := StackG {
   stack_tokG :: inG (exclR unitO) Γ;
